\documentclass{extarticle}
\usepackage[utf8]{inputenc}
\usepackage{amsmath}
\usepackage{amssymb}
\usepackage{graphicx}
\usepackage[vcentering,dvips]{geometry}
\geometry{papersize={19cm,16cm},total={16.5cm,8cm}}
%\graphicspath{{./Rigan/}}
%\renewcommand{\baselinestretch}{1.5}
%\addtolength{\oddsidemargin}{1in}
%\addtolength{\evensidemargin}{1.5in}
%\addtolength{\textwidth}{1.9in}

\addtolength{\topmargin}{0in}
\addtolength{\textheight}{-0.5in} 

\setlength{\parindent}{0em}

\date{}
\begin{document}
	

	%\begin{enumerate}
	
		 \textbf{Soal. } Untuk sembarang bilangan real positif $a,b,c$, buktikan bahwa 
		 $$\left(\dfrac{a}{a+2b} \right)^2+\left(\dfrac{b}{b+2c} \right)^2+\left(\dfrac{c}{c+2a} \right)^2 \ge \dfrac{1}{3}$$
	%\end{enumerate}
	
	\newpage
	
	\textbf{Soal. } Untuk sembarang bilangan real positif $a,b,c$, buktikan bahwa 
	$$\left(\dfrac{a}{a+2b} \right)^2+\left(\dfrac{b}{b+2c} \right)^2+\left(\dfrac{c}{c+2a} \right)^2 \ge \dfrac{1}{3}$$
	\textbf{Solusi. }
	\begin{align*}
		\sum_{cyc} \left(\dfrac{a}{a+2b} \right)^2 
		 &\overset{QM-AM}{\ge} 3\left(\dfrac{1}{3}\sum_{cyc} \left(\dfrac{a}{a+2b} \right)\right)^2
		 = \dfrac{1}{3}\left(\sum_{cyc} \left(\dfrac{a}{a+2b} \right)\right)^2\\
		 &\overset{CS-Engel}{\ge} \dfrac{1}{3}\left(\dfrac{\left(\sum_{cyc}a\right)^2}{\left(\sum_{cyc}a(a+2b)\right)} \right)^2
		 = \dfrac{1}{3}\left(\dfrac{\left(\sum_{cyc}a\right)^2}{\left(\sum_{cyc}a^2+\sum_{cyc}2ab\right)} \right)^2
		 = \dfrac{1}{3}(1)^2 = \dfrac{1}{3}
	\end{align*}
	Dengan kesamaan terjadi saat $a=b=c$.
	$$$$
\end{document}
